Refactored the file Sort.v into LinDec.v (about decidable linear orders) and Sorted.v (about sortedness, counting, permutations). Put all the list functions and lemmas in a separate file. Renamed nb_occ to count. Proved a few lemmas about count and one about perm. Refactored all files with sorting algorithms — removed the thrash and moved lemmas and auxiliary functions elsewhere. The build passes.

Sorting/Mergesort.v
@@ -1,6 +1,12 @@
 Add Rec LoadPath "/home/zeimer/Code/Coq".
 
+Require Import Coq.Program.Wf.
+Require Import Recdef.
+
+Require Import Div2.
+
 Require Import Sort.
+Require Import ListLemmas.
 
 Set Implicit Arguments.
 
@@ -10,80 +16,23 @@ Fixpoint merge (A : LinDec) (l1 : list A) {struct l1} : list A -> list A :=
         | [], _ => l2
         | _, [] => l1
         | h1 :: t1, h2 :: t2 =>
-            if @leq_total_dec A h1 h2
+            if h1 <=? h2
             then h1 :: merge A t1 l2
             else h2 :: f t2
     end.
 
-Hint Constructors sorted.
-
-Theorem merge_sorted : forall (A : LinDec) (l1 l2 : list A),
+(* TODO *) Theorem merge_sorted : forall (A : LinDec) (l1 l2 : list A),
     sorted A l1 -> sorted A l2 -> sorted A (merge A l1 l2).
 Proof.
   intros A l1 l2 H. generalize dependent l2.
   induction H.
     destruct l2; auto.
+    induction 1; simpl in *; dec.
     induction 1.
       simpl. auto.
-      simpl. destruct (leq_total_dec x x0); auto.
-      simpl in *. destruct (leq_total_dec x x0); auto.
-        destruct (leq_total_dec x y); auto.
-    induction 1.
-      simpl. auto.
-      specialize (IHsorted _ (sorted1 A x0)). simpl in *.
-        destruct (leq_total_dec x x0); auto.
-          destruct (leq_total_dec y x0); simpl; auto.
-      simpl. destruct (leq_total_dec x x0).
+      specialize (IHsorted _ (sorted1 A x0)). simpl in *. dec.
+      simpl.
 Abort.
-
-Fixpoint take {A : Type} (n : nat) (l : list A) : list A :=
-match n, l with
-    | 0, _ => []
-    | _, [] => []
-    | S n', h :: t => h :: take n' t
-end.
-
-Fixpoint drop {A : Type} (n : nat) (l : list A) : list A :=
-match n, l with
-    | 0, _ => l
-    | _, [] => []
-    | S n', h :: t => drop n' t
-end.
-
-Theorem take_length : forall (A : Type) (n : nat) (l : list A),
-    length (take n l) <= length l.
-Proof.
-  induction n as [| n']; destruct l; simpl; intros; auto.
-    omega.
-    apply le_n_S. apply IHn'.
-Qed.
-
-Theorem take_length2 : forall (A : Type) (n : nat) (l : list A),
-    n < length l -> length (take n l) < length l.
-Proof.
-  induction n as [| n']; simpl; intros; auto.
-  destruct l; simpl in *.
-    inversion H.
-    apply lt_n_S. apply IHn'. omega.
-Qed.
-
-Theorem drop_length : forall (A : Type) (l : list A) (n : nat),
-    length (drop n l) <= length l.
-Proof.
-  induction l as [| h t]; destruct n; simpl; intros; auto.
-Qed.
-
-Theorem drop_length2 : forall (A : Type) (l : list A) (n : nat),
-    0 < n -> l <> [] -> length (drop n l) < length l.
-Proof.
-  induction l as [| h t]; intros; destruct n; try (inversion H; fail);
-  simpl in *.
-    contradiction H0. trivial.
-    unfold lt. apply le_n_S. apply drop_length.
-Qed.
-
-Require Import Arith.
-Require Import Div2.
 
 (* Mergesort using Program Fixpoint. *)
 Program Fixpoint msPF (A : LinDec) (l : list A) 
@@ -98,10 +47,10 @@ match l with
       merge A (msPF A l1) (msPF A l2)
 end.
 Next Obligation.
-  apply take_length2. apply lt_div2. destruct l; simpl;
+  apply take_length_lt. apply lt_div2. destruct l; simpl;
   try (contradiction H0; auto; fail); try omega. Qed.
 Next Obligation.
-  apply drop_length2; auto.
+  apply drop_length_lt; auto.
     destruct l; simpl. contradiction H0; auto.
       destruct l; simpl. contradiction (H c); auto. omega. Qed.
 Next Obligation.
@@ -122,8 +71,8 @@ match l with
       merge A (msFun A l1) (msFun A l2)
 end.
 Proof.
-  intros. apply drop_length2; simpl. omega. inversion 1.
-  intros. apply take_length2. apply lt_div2. simpl. omega.
+  intros. apply drop_length_lt; simpl. omega. inversion 1.
+  intros. apply take_length_lt. apply lt_div2. simpl. omega.
 Defined.
 
 Eval compute in msFun natle testl.
@@ -157,14 +106,13 @@ match l with
 end)).
 Proof.
   all: unfold l1, l2, n.
-    apply take_length2. apply lt_div2. simpl. omega.
-    apply drop_length2; simpl.
+    apply take_length_lt. apply lt_div2. simpl. omega.
+    apply drop_length_lt; simpl.
       omega.
       inversion 1.
 Defined.
 
 (* Mergesort using Bove-Capretta *)
-
 Inductive msDom {A : LinDec} : list A -> Type :=
     | msDom0 : msDom []
     | msDom1 : forall x : A, msDom [x]
@@ -186,8 +134,8 @@ Proof.
   intro. apply well_founded_induction_type with lengthOrder.
     apply lengthOrder_wf.
     intros l ms. destruct l as [| h [| h' t]]; constructor.
-      apply ms. apply take_length2. apply lt_div2. simpl. omega.
-      apply ms. apply drop_length2. simpl. omega. inversion 1.
+      apply ms. apply take_length_lt. apply lt_div2. simpl. omega.
+      apply ms. apply drop_length_lt. simpl. omega. inversion 1.
 Defined.
 
 Definition msBC (A : LinDec) (l : list A) : list A :=
