Sorting/InsertionSort.v
@@ -1,0 +1,59 @@
+Add Rec LoadPath "/home/zeimer/Code/Coq".
+
+Require Import Sort.
+
+Set Implicit Arguments.
+
+Fixpoint ins (A : LinDec) (x : A) (l : list A) : list A :=
+match l with
+    | [] => [x]
+    | h :: t => if x <=? h then x :: h :: t else h :: (ins A x t)
+end.
+
+Definition insertionSort (A : LinDec) (l : list A)
+    : list A := fold_right (ins A) [] l.
+
+Eval compute in insertionSort natle testl.
+
+Lemma perm_ins: forall (A : LinDec) (x : A) (l : list A),
+    perm A (x :: l) (ins A x l).
+Proof.
+  unfold perm; intros. induction l.
+    reflexivity.
+    unfold ins; destruct (leqb x a); fold ins.
+      reflexivity.
+      rewrite (perm_swap A x a l l (perm_refl A l)).
+        simpl. rewrite <- IHl. reflexivity.
+Qed.
+
+Lemma ins_sorted : forall (A : LinDec) (x : A) (l : list A),
+    sorted A l -> sorted A (ins A x l).
+Proof.
+  induction l as [| h t]; intros; simpl.
+    constructor.
+    destruct (leqb_spec x h).
+      auto.
+      induction t as [| h' t']; simpl in *.
+        repeat constructor.
+          destruct (leq_total h x); auto.
+        destruct (leqb_spec x h'); intros.
+          constructor.
+            destruct (leq_total x h); auto.
+            constructor. eauto. eapply sorted_tail. eauto.
+            constructor.
+              inversion H. auto.
+              apply IHt; auto. eapply sorted_tail; eauto.
+Qed.
+
+Instance Sort_insertionSort : Sort :=
+{
+    sort := insertionSort
+}.
+Proof.
+  induction l as [| h t]; simpl; auto.
+    apply ins_sorted. assumption.
+  induction l as [| h t]; simpl; auto.
+    apply perm_trans with (h :: insertionSort A t); auto. apply perm_ins.
+Defined.
+
+Eval cbv in sort testl.
