Sorting/LinDec.v
@@ -1,0 +1,112 @@
+Require Export List.
+Export ListNotations.
+
+Require Export Bool.Bool.
+Require Export Arith.
+Require Export Omega.
+
+Class LinDec : Type :=
+{
+    carrier : Type;
+    leq : carrier -> carrier -> Prop;
+    leq_refl : forall x : carrier, leq x x;
+    leq_antisym : forall x y : carrier, leq x y -> leq y x -> x = y;
+    leq_trans : forall x y z : carrier, leq x y -> leq y z -> leq x z;
+    leq_total : forall x y : carrier, leq x y \/ leq y x;
+    leqb : carrier -> carrier -> bool;
+    leqb_spec : forall x y : carrier, reflect (leq x y) (leqb x y)
+}.
+
+Coercion carrier : LinDec >-> Sortclass.
+
+Infix "≤" := leq (at level 70).
+Infix "<=?" := leqb (at level 70).
+
+Hint Resolve leq_refl leq_antisym leq_trans leq_total.
+Hint Constructors reflect.
+
+Definition LinDec_eqb {A : LinDec} (x y : A) : bool :=
+    andb (leqb x y) (leqb y x).
+
+Infix "=?" := LinDec_eqb (at level 70).
+
+Definition LinDec_eq_dec : forall {A : LinDec} (x y : A),
+    {x = y} + {x <> y}.
+Proof.
+  intros. destruct (leqb_spec x y) as [H1 | H1], (leqb_spec y x) as [H2 | H2].
+    left; apply leq_antisym; auto.
+    right. intro. apply H2. subst. auto.
+    right. intro. apply H1. subst. auto.
+    cut False.
+      inversion 1.
+      destruct (leq_total x y); contradiction.
+Defined.
+
+Theorem LinDec_eqb_spec :
+  forall (A : LinDec) (x y : A), reflect (x = y) (x =? y).
+Proof.
+  unfold LinDec_eqb. intros.
+  destruct (LinDec_eq_dec x y); subst.
+    destruct (leqb_spec y y); simpl; auto.
+    destruct (leqb_spec x y); simpl; auto.
+      destruct (leqb_spec y x); simpl; auto.
+Defined.
+
+Ltac dec := simpl; repeat
+match goal with
+    | |- context [?x =? ?y] => destruct (LinDec_eqb_spec _ x y); subst; intros
+    | |- context [?x <=? ?y] => destruct (leqb_spec x y); intros
+end; simpl; try
+match goal with
+    | H : ?x <> ?x |- _ => contradiction H; reflexivity
+end; auto; try omega.
+
+Lemma LinDec_not_leq : forall (A : LinDec) (x y : A),
+    ~ leq x y -> leq y x.
+Proof.
+  intros. destruct (leqb_spec y x).
+    assumption.
+    cut False.
+      inversion 1.
+      destruct (leq_total x y); contradiction.
+Defined.
+
+Hint Resolve LinDec_not_leq.
+
+Instance natle : LinDec :=
+{
+    carrier := nat;
+    leq := le;
+    leqb := leb
+}.
+Proof.
+  intros. apply le_n.
+  intros. apply le_antisym; auto.
+  intros. eapply le_trans; eauto.
+  intros. destruct (le_gt_dec x y) as [H | H].
+    left. auto.
+    right. unfold lt in H. apply le_Sn_le. auto.
+  intros. case_eq (leb x y); intro.
+    apply leb_complete in H. auto.
+    apply leb_complete_conv in H. constructor. omega.
+Defined.
+
+Definition testl := [3; 0; 1; 42; 34; 19; 44; 21; 42; 65; 5].
+
+Definition min_dflt (A : LinDec) (d : A) (l : list A) : A :=
+    fold_right (fun x y => if x <=? y then x else y) d l.
+
+Theorem min_In :
+  forall (A : LinDec) (h : A) (t : list A),
+    In (min_dflt A h t) (h :: t).
+Proof.
+  induction t as [| h' t'].
+    simpl. left. reflexivity.
+    inversion IHt'.
+      simpl. destruct (h' <=? _).
+        right. left. reflexivity.
+        left. assumption.
+      simpl. destruct (h' <=? _).
+        right. left. reflexivity.
+        right. right. assumption.
+Qed.
