Sorting/ListLemmas.v
@@ -1,0 +1,106 @@
+Add Rec LoadPath "/home/zeimer/Code/Coq".
+
+Require Import LinDec.
+
+Definition lengthOrder {A : Type} (l1 l2 : list A) : Prop :=
+    length l1 < length l2.
+
+Theorem lengthOrder_wf : forall (A : Type),
+    well_founded (@lengthOrder A).
+Proof.
+  unfold lengthOrder. intro.
+  apply (@well_founded_lt_compat _ (@length A)). trivial.
+Defined.
+
+Fixpoint remove_once {A : LinDec} (x : A) (l : list A) : list A :=
+match l with
+    | [] => []
+    | h :: t => if x =? h then t else h :: remove_once x t
+end.
+
+Lemma remove_once_In_eq : forall (A : LinDec) (x : A) (l : list A),
+    In x l -> S (length (remove_once x l)) = length l.
+Proof.
+  induction l as [| h t]; destruct 1; dec.
+Defined.
+
+Lemma remove_once_le : forall (A : LinDec) (x : A) (l : list A),
+    length (remove_once x l) <= length l.
+Proof.
+  induction l as [| h t]; dec.
+Defined.
+
+Lemma remove_once_In_lt : forall (A : LinDec) (x : A) (l : list A),
+    In x l -> length (remove_once x l) < length l.
+Proof.
+  induction l as [| h t]; destruct 1; dec.
+    apply lt_n_S. auto.
+Defined.
+
+Lemma remove_once_min_lengthOrder :
+  forall (A : LinDec) (h : A) (t : list A),
+    lengthOrder (remove_once (min_dflt A h t) (h :: t)) (h :: t).
+Proof.
+  red; intros. apply remove_once_In_lt. apply min_In.
+Defined.
+
+Lemma filter_length :
+  forall (A : Type) (f : A -> bool) (l : list A),
+    length (filter f l) <= length l.
+Proof.
+  induction l as [| h t]; simpl; try destruct (f h); simpl; omega.
+Qed.
+
+Lemma filter_lengthOrder :
+  forall {A : Type} (p : A -> bool) (h : A) (t : list A),
+    lengthOrder (filter p t) (h :: t).
+Proof.
+  intros. unfold lengthOrder, lt. simpl. apply le_n_S.
+  apply filter_length.
+Qed.
+
+Fixpoint take {A : Type} (n : nat) (l : list A) : list A :=
+match n, l with
+    | 0, _ => []
+    | _, [] => []
+    | S n', h :: t => h :: take n' t
+end.
+
+Fixpoint drop {A : Type} (n : nat) (l : list A) : list A :=
+match n, l with
+    | 0, _ => l
+    | _, [] => []
+    | S n', h :: t => drop n' t
+end.
+
+Theorem take_length_le : forall (A : Type) (n : nat) (l : list A),
+    length (take n l) <= length l.
+Proof.
+  induction n as [| n']; destruct l; simpl; intros; auto.
+    omega.
+    apply le_n_S. apply IHn'.
+Qed.
+
+Theorem take_length_lt : forall (A : Type) (n : nat) (l : list A),
+    n < length l -> length (take n l) < length l.
+Proof.
+  induction n as [| n']; simpl; intros; auto.
+  destruct l; simpl in *.
+    inversion H.
+    apply lt_n_S. apply IHn'. omega.
+Qed.
+
+Theorem drop_length_le : forall (A : Type) (l : list A) (n : nat),
+    length (drop n l) <= length l.
+Proof.
+  induction l as [| h t]; destruct n; simpl; intros; auto.
+Qed.
+
+Theorem drop_length_lt : forall (A : Type) (l : list A) (n : nat),
+    0 < n -> l <> [] -> length (drop n l) < length l.
+Proof.
+  induction l as [| h t]; intros; destruct n; try (inversion H; fail);
+  simpl in *.
+    contradiction H0. trivial.
+    unfold lt. apply le_n_S. apply drop_length_le.
+Qed.
