Sorting/Quicksort.v
@@ -1,24 +1,12 @@
 Add Rec LoadPath "/home/zeimer/Code/Coq".
 
+Require Import Coq.Program.Wf.
+Require Import Recdef.
+
 Require Import Sort.
+Require Import ListLemmas.
 
-Theorem filter_length : forall (A : Type) (f : A -> bool) (l : list A),
-    length (filter f l) <= length l.
-Proof.
-  induction l as [| h t]; simpl; try destruct (f h); simpl; omega.
-Qed.
-
-Theorem filter_comm : forall (A : Type) (l : list A) (f g : A -> bool),
-    filter f (filter g l) = filter g (filter f l).
-Proof.
-  induction l as [| h t]; intros.
-    simpl. trivial.
-    simpl. case_eq (f h); case_eq (g h); intros; simpl.
-      rewrite H, H0, IHt. trivial.
-      rewrite H, IHt. trivial.
-      rewrite H0, IHt. trivial.
-      rewrite IHt. trivial.
-Qed.
+Set Implicit Arguments.
 
 Hint Resolve le_n_S filter_length.
 
@@ -49,33 +37,7 @@ Defined.
 
 Eval compute in qsFun natle testl.
 
-Lemma sorted_inv2 :
-  forall (A : LinDec) (x y : A) (l : list A),
-    sorted A (x :: y :: l) -> leq x y.
-Proof.
-  inversion 1; subst. assumption.
-Qed.
-
-Lemma sorted_app_all :
-  forall (A : LinDec) (l : list A) (h : A) (t : list A),
-    sorted A l -> sorted A (h :: t) -> (forall x : A, In x l -> leq x h) ->
-      sorted A (l ++ h :: t).
-Proof.
-  induction l as [| h t]; simpl; intros.
-    assumption.
-    destruct t as [| h' t'].
-      simpl in *. constructor.
-        eapply (H1 h); eauto.
-        assumption.
-      rewrite <- app_comm_cons. constructor.
-        eapply sorted_inv2. eassumption.
-        apply IHt.
-          apply sorted_inv with h. assumption.
-          assumption.
-          intros. apply H1. right. assumption.
-Qed.
-
-Theorem qsFun_sorted :
+(* TODO *) Theorem qsFun_sorted :
   forall (A : LinDec) (l : list A), sorted A (qsFun A l).
 Proof.
   intros. functional induction (@qsFun A) l.
@@ -83,7 +45,7 @@ Proof.
     apply sorted_app_all.
       assumption.
       Focus 2. intros.
-Abort. (* TODO : *)
+Abort.
 
 (* Quicksort using fuel recursion. *)
 Fixpoint qsFuel' (A : LinDec) (fuel : nat) (l : list A) : list A :=
@@ -102,15 +64,6 @@ Definition qsFuel (A : LinDec) (l : list A) : list A :=
 Eval compute in (qsFuel natle testl).
 
 (* Quicksort using well-founded recursion. *)
-
-Lemma filter_lengthOrder :
-  forall {A : Type} (p : A -> bool) (h : A) (t : list A),
-    lengthOrder (filter p t) (h :: t).
-Proof.
-  intros. unfold lengthOrder, lt. simpl. apply le_n_S.
-  apply filter_length.
-Qed.
-
 Definition qsWf (A : LinDec) : list A -> list A.
 Proof.
   apply (Fix (@lengthOrder_wf A) _).
@@ -127,7 +80,6 @@ Defined.
 Eval compute in qsWf natle testl.
 
 (* Quicksort using wel-founded recursion and refine. *)
-
 Definition qsWfRef (A : LinDec) : list A -> list A.
 refine (Fix (@lengthOrder_wf A) _ (fun (l : list A) =>
 match l with
@@ -144,9 +96,6 @@ Defined.
 Eval compute in qsWfRef natle testl.
 
 (* Quicksort using Bove-Capretta *)
-
-Require Import Coq.Init.Wf.
-
 Inductive qsDom {A : LinDec} : list A -> Type :=
     | qsDom0 : qsDom nil
     | qsDom1 : forall (h : A) (t : list A),
@@ -154,12 +103,11 @@ Inductive qsDom {A : LinDec} : list A -> Type :=
         qsDom (filter (fun x : A => negb (leqb x h)) t) ->
         qsDom (h :: t).
 
-Fixpoint qsBC' (A : LinDec) (l : list A) (dom : qsDom l) : list A :=
+Fixpoint qsBC' {A : LinDec} (l : list A) (dom : qsDom l) : list A :=
 match dom with
     | qsDom0 => nil
     | qsDom1 h t dom1 dom2 =>
-        qsBC' A (filter (fun x : A => leqb x h) t) dom1 ++ h ::
-        qsBC' A (filter (fun x : A => negb (leqb x h)) t) dom2
+        qsBC' dom1 ++ h :: qsBC' dom2
 end.
 
 Theorem all_qsDom : forall (A : LinDec) (l : list A), qsDom l.
@@ -172,43 +120,6 @@ Proof.
 Defined.
 
 Definition qsBC (A : LinDec) (l : list A) : list A :=
-    qsBC' A l (all_qsDom A l).
+    @qsBC' A l (all_qsDom A l).
 
 Eval compute in qsBC natle testl.
-
-(* nb_occ lemmas *)
-
-Lemma nb_occ_reverse :
-  forall (A : LinDec) (l : list A) (x : A),
-    nb_occ A x (rev l) = nb_occ A x l.
-Proof.
-  induction l as [| h t].
-    simpl; intros; reflexivity.
-    intros. SearchAbout rev_append. rewrite rev_alt. simpl.
-Abort.
-
-(* Tried to prove that quicksort gives a permutation, but failed. *)
-Lemma nb_occ_app : forall (A : LinDec) (x : A) (l1 l2 l3 : list A),
-    l3 = l1 ++ l2 -> nb_occ A x (l1 ++ l2) = nb_occ A x (l2 ++ l1).
-Proof.
-  induction l1 as [| h1 t1].
-    simpl; intros. rewrite app_nil_r. reflexivity.
-    intros. rewrite <- app_comm_cons at 1.
-      replace (l2 ++ h1 :: t1) with ((l2 ++ [h1]) ++ t1). (*
-        rewrite <- IHt1. simpl. destruct (LinDec_eq x h1).*)
-Restart. Check well_founded_induction.
-  intros A x l1 l2.
-  apply (@well_founded_induction (list A) _ (lengthOrder_wf A)
-    (fun l3 => l3 = l1 ++ l2 -> nb_occ A x (l1 ++ l2) = nb_occ A x (l2 ++ l1))).
-  intros; subst.
-Abort.
-
-Lemma perm_app : forall (A : LinDec) (l1 l2 : list A),
-    perm A (l1 ++ l2) (l2 ++ l1).
-Proof.
-  induction l1 as [| h t].
-    simpl. intro. rewrite app_nil_r. apply perm_refl.
-    simpl. induction l2 as [| h' t'].
-      simpl. rewrite app_nil_r. apply perm_refl.
-      simpl.
-Abort.
