make_makefile.sh
@@ -1,3 +1,3 @@
 #!/bin/sh
 
-coq_makefile -R "." Rand -o makefile *v
+coq_makefile -R "." RandomCoqCode -o makefile Sorting/*v Reification/*v
