rebuild.sh
@@ -1,5 +1,5 @@
 #!/bin/sh
 
 make clean
-./make_makefile
+./make_makefile.sh
 make
